NormalizeAst.dfy
@@ -75,16 +75,16 @@ module NormalizeAst {
       (Some(SeqSimpleOptCmd(precedingSimple, Loop(invs, body') )), None)
   }
 
-  lemma TransformAstCorrectness<A(!new)>(a: absval_interp<A>, c: Cmd, precedingSimple: Option<SimpleCmd>, post: WpPostShallow<A>, s: state<A>)
+  lemma TransformAstCorrectness<A(!new)>(a: absval_interp<A>, c: Cmd, precedingSimple: Option<SimpleCmd>, post: WpPost<A>, s: state<A>)
     requires LabelsWellDefAux(SeqSimpleOptCmd(precedingSimple, c), post.scopes.Keys)
     requires var (cOpt', scExitOpt):= NormalizeAst(c, precedingSimple);
              LabelsWellDefAux(SeqCmdSimpleOpt(cOpt', scExitOpt), post.scopes.Keys)
     ensures 
       var (cOpt', scExitOpt):= NormalizeAst(c, precedingSimple);
-      WpShallow(a, SeqSimpleOptCmd(precedingSimple, c), post)(s) == 
-      WpShallow(a, SeqCmdSimpleOpt(cOpt', scExitOpt), post)(s)
+      WpCmd(a, SeqSimpleOptCmd(precedingSimple, c), post)(s) == 
+      WpCmd(a, SeqCmdSimpleOpt(cOpt', scExitOpt), post)(s)
   {
-    reveal WpShallow();
+    reveal WpCmd();
 
     var (cOpt', scExitOpt):= NormalizeAst(c, precedingSimple);
 
@@ -94,35 +94,35 @@ module NormalizeAst {
     case Seq(c1, c2) => 
       var (c1Opt', scExitOpt1) := NormalizeAst(c1, precedingSimple);
       var (c2Opt', scExitOpt2) := NormalizeAst(c2, scExitOpt1);
-      var post2 := WpShallow(a, c2, post);
+      var post2 := WpCmd(a, c2, post);
 
       calc {
-        WpShallow(a, SeqSimpleOptCmd(precedingSimple, Seq(c1,c2)), post)(s); 
-        WpShallow(a, SeqSimpleOptCmd(precedingSimple, c1), WpPostShallow(post2, post.currentScope, post.scopes))(s); //IH1
-          { TransformAstCorrectness(a, c1, precedingSimple, WpPostShallow(post2, post.currentScope, post.scopes), s); }
-        WpShallow(a, SeqCmdSimpleOpt(c1Opt', scExitOpt1), WpPostShallow(post2, post.currentScope, post.scopes))(s);
+        WpCmd(a, SeqSimpleOptCmd(precedingSimple, Seq(c1,c2)), post)(s); 
+        WpCmd(a, SeqSimpleOptCmd(precedingSimple, c1), WpPost(post2, post.currentScope, post.scopes))(s); //IH1
+          { TransformAstCorrectness(a, c1, precedingSimple, WpPost(post2, post.currentScope, post.scopes), s); }
+        WpCmd(a, SeqCmdSimpleOpt(c1Opt', scExitOpt1), WpPost(post2, post.currentScope, post.scopes))(s);
       }
 
       if c1Opt'.Some? {
-        var p := WpPostShallow(WpShallow(a, SeqSimpleOptCmd(scExitOpt1, c2), post), post.currentScope, post.scopes);
-        var q := WpPostShallow(WpShallow(a, SeqCmdSimpleOpt(c2Opt', scExitOpt2), post), post.currentScope, post.scopes);
+        var p := WpPost(WpCmd(a, SeqSimpleOptCmd(scExitOpt1, c2), post), post.currentScope, post.scopes);
+        var q := WpPost(WpCmd(a, SeqCmdSimpleOpt(c2Opt', scExitOpt2), post), post.currentScope, post.scopes);
 
         calc {
-          WpShallow(a, SeqCmdSimpleOpt(c1Opt', scExitOpt1), WpPostShallow(post2, post.currentScope, post.scopes))(s);
-          WpShallow(a, c1Opt'.value, p)(s); 
+          WpCmd(a, SeqCmdSimpleOpt(c1Opt', scExitOpt1), WpPost(post2, post.currentScope, post.scopes))(s);
+          WpCmd(a, c1Opt'.value, p)(s); 
             { 
               forall s' | true 
-              ensures WpShallow(a, SeqSimpleOptCmd(scExitOpt1, c2), post)(s') ==
-                      WpShallow(a, SeqCmdSimpleOpt(c2Opt', scExitOpt2), post)(s')
+              ensures WpCmd(a, SeqSimpleOptCmd(scExitOpt1, c2), post)(s') ==
+                      WpCmd(a, SeqCmdSimpleOpt(c2Opt', scExitOpt2), post)(s')
               {
                 TransformAstCorrectness(a, c2, scExitOpt1, post, s');
               }
 
-              WpShallowPointwise(a, c1Opt'.value, p, q, s);
+              WpCmdPointwise(a, c1Opt'.value, p, q, s);
             }//IH2 + WP pointwise
-          WpShallow(a, c1Opt'.value, q)(s);
-          WpShallow(a, Seq(c1Opt'.value, SeqCmdSimpleOpt(c2Opt', scExitOpt2)), post)(s);
-          WpShallow(a, SeqCmdSimpleOpt(SeqCmdOpt(c1Opt', c2Opt'), scExitOpt2), post)(s);
+          WpCmd(a, c1Opt'.value, q)(s);
+          WpCmd(a, Seq(c1Opt'.value, SeqCmdSimpleOpt(c2Opt', scExitOpt2)), post)(s);
+          WpCmd(a, SeqCmdSimpleOpt(SeqCmdOpt(c1Opt', c2Opt'), scExitOpt2), post)(s);
         }
       } else {
           TransformAstCorrectness(a, c2, scExitOpt1, post, s);
@@ -132,7 +132,7 @@ module NormalizeAst {
       var bodyNew := SeqCmdSimpleOpt(body', scExitOpt);
       var updatedScopes := if optLabel.Some? then post.scopes[optLabel.value := post.normal] else post.scopes;
 
-      var post' := WpPostShallow(post.normal, post.normal, updatedScopes);
+      var post' := WpPost(post.normal, post.normal, updatedScopes);
       var updatedPost := prevState => ResetVarsPost(varDecls, post', prevState);
 
       assert updatedScopes.Keys == if optLabel.Some? then {optLabel.value} + post.scopes.Keys else post.scopes.Keys;
@@ -146,7 +146,7 @@ module NormalizeAst {
       { }
 
       forall s',sPrev | true
-      ensures WpShallow(a, body, updatedPost(sPrev))(s') == WpShallow(a, bodyNew, updatedPost(sPrev))(s')
+      ensures WpCmd(a, body, updatedPost(sPrev))(s') == WpCmd(a, bodyNew, updatedPost(sPrev))(s')
       {
 
         assert updatedPost(sPrev).scopes.Keys == if optLabel.Some? then {optLabel.value} + post.scopes.Keys else post.scopes.Keys;
@@ -154,32 +154,32 @@ module NormalizeAst {
       }
 
       forall s' | true
-        ensures ForallVarDeclsShallow(a, varDecls, WpShallow(a, body, updatedPost(s')))(s') == ForallVarDeclsShallow(a, varDecls, WpShallow(a, bodyNew, updatedPost(s')))(s')
+        ensures ForallVarDecls(a, varDecls, WpCmd(a, body, updatedPost(s')))(s') == ForallVarDecls(a, varDecls, WpCmd(a, bodyNew, updatedPost(s')))(s')
       {
-        assert forall s' :: WpShallow(a, body, updatedPost(s'))(s') == WpShallow(a, bodyNew, updatedPost(s'))(s');
-        ForallVarDeclsPointwise(a, varDecls,  WpShallow(a, body, updatedPost(s')), WpShallow(a, bodyNew, updatedPost(s')), s');
+        assert forall s' :: WpCmd(a, body, updatedPost(s'))(s') == WpCmd(a, bodyNew, updatedPost(s'))(s');
+        ForallVarDeclsPointwise(a, varDecls,  WpCmd(a, body, updatedPost(s')), WpCmd(a, bodyNew, updatedPost(s')), s');
       }
 
       var c' := SeqSimpleOptCmd(precedingSimple, Scope(optLabel, varDecls, bodyNew));
 
       forall s' | true
-      ensures WpShallow(a, Scope(optLabel, varDecls, body), post)(s') == WpShallow(a, Scope(optLabel, varDecls, bodyNew), post)(s')
+      ensures WpCmd(a, Scope(optLabel, varDecls, body), post)(s') == WpCmd(a, Scope(optLabel, varDecls, bodyNew), post)(s')
       {
         calc {
-          WpShallow(a, Scope(optLabel, varDecls, body), post)(s');
-          ForallVarDeclsShallow(a, varDecls, WpShallow(a, body, updatedPost(s')))(s');
+          WpCmd(a, Scope(optLabel, varDecls, body), post)(s');
+          ForallVarDecls(a, varDecls, WpCmd(a, body, updatedPost(s')))(s');
         }
       }
       
       if(precedingSimple.Some?) {
-        var post1 := WpPostShallow(WpShallow(a, c, post), post.currentScope, post.scopes);
-        var post2 := WpPostShallow(WpShallow(a, Scope(optLabel, varDecls, bodyNew), post), post.currentScope, post.scopes);
+        var post1 := WpPost(WpCmd(a, c, post), post.currentScope, post.scopes);
+        var post2 := WpPost(WpCmd(a, Scope(optLabel, varDecls, bodyNew), post), post.currentScope, post.scopes);
         calc {
-          WpShallow(a, Seq(SimpleCmd(precedingSimple.value), c), post)(s);
-          WpShallow(a, SimpleCmd(precedingSimple.value), post1)(s); 
+          WpCmd(a, Seq(SimpleCmd(precedingSimple.value), c), post)(s);
+          WpCmd(a, SimpleCmd(precedingSimple.value), post1)(s); 
           { 
-            WpShallowPointwise(a, SimpleCmd(precedingSimple.value), post1, post2, s); }
-          WpShallow(a, SimpleCmd(precedingSimple.value), post2)(s);
+            WpCmdPointwise(a, SimpleCmd(precedingSimple.value), post1, post2, s); }
+          WpCmd(a, SimpleCmd(precedingSimple.value), post2)(s);
         }
       }     
     case If(condOpt, thn, els) =>
@@ -190,19 +190,19 @@ module NormalizeAst {
 
       forall s' | true 
       ensures 
-        WpShallow(a, If(condOpt, thn, els), post)(s') == WpShallow(a, If(condOpt, thn', els'), post)(s')
+        WpCmd(a, If(condOpt, thn, els), post)(s') == WpCmd(a, If(condOpt, thn', els'), post)(s')
       {
           TransformAstCorrectness(a, thn, None, post, s');
           TransformAstCorrectness(a, els, None, post, s');
       }
 
       if precedingSimple.Some? {
-        var post1 := WpPostShallow(WpShallow(a, If(condOpt, thn, els), post), post.currentScope, post.scopes);
-        var post2 := WpPostShallow(WpShallow(a, If(condOpt, thn', els'), post), post.currentScope, post.scopes);
+        var post1 := WpPost(WpCmd(a, If(condOpt, thn, els), post), post.currentScope, post.scopes);
+        var post2 := WpPost(WpCmd(a, If(condOpt, thn', els'), post), post.currentScope, post.scopes);
         calc {
-          WpShallow(a, SimpleCmd(precedingSimple.value), post1)(s);
-            { WpShallowPointwise(a, SimpleCmd(precedingSimple.value), post1, post2, s); }
-          WpShallow(a, SimpleCmd(precedingSimple.value), post2)(s);
+          WpCmd(a, SimpleCmd(precedingSimple.value), post1)(s);
+            { WpCmdPointwise(a, SimpleCmd(precedingSimple.value), post1, post2, s); }
+          WpCmd(a, SimpleCmd(precedingSimple.value), post2)(s);
         }
       }      
     case _ => assume false;
