RemoveScopedVarsProof.dfy
@@ -15,13 +15,13 @@ module MakeScopedVarsUniqueProof {
   import opened MakeScopedVarsUniqueImpl
   import opened Naming
 
-  lemma RelStateRemoveScopedVarsCorrect<A(!new)>(a: absval_interp<A>, c: Cmd, post: WpPostShallow<A>)
+  lemma RelStateRemoveScopedVarsCorrect<A(!new)>(a: absval_interp<A>, c: Cmd, post: WpPost<A>)
     requires 
       var (c', decls) := RemoveScopedVars(c);
       LabelsWellDefAux(c, post.scopes.Keys) && LabelsWellDefAux(c', post.scopes.Keys)
     ensures 
       var (c', decls) := RemoveScopedVars(c);
-      forall s :: WpShallow(a, c, post)(s) == ForallVarDeclsShallow(a, decls, WpShallow(a, c', ResetVarsPost(decls, post, s)))(s)
+      forall s :: WpCmd(a, c, post)(s) == ForallVarDecls(a, decls, WpCmd(a, c', ResetVarsPost(decls, post, s)))(s)
     /* almost the same as Scope(None, decls, body)
       Main difference is that currentScope is not updated.
       If show that body has no direct breaks, then it would be the same
